<?xml version="1.0" encoding="utf-8"?>
<rdf:RDF
   xmlns:dcterms="http://purl.org/dc/terms/"
   xmlns:owl="http://www.w3.org/2002/07/owl#"
   xmlns:rdf="http://www.w3.org/1999/02/22-rdf-syntax-ns#"
   xmlns:rdfs="http://www.w3.org/2000/01/rdf-schema#"
   xmlns:skos="http://www.w3.org/2004/02/skos/core#"
   xmlns:vann="http://purl.org/vocab/vann/"
>
  <rdf:Description rdf:about="http://data.europa.eu/a4g/ontology#core">
    <rdf:type rdf:resource="http://www.w3.org/2002/07/owl#Ontology"/>
    <owl:imports rdf:resource="http://xmlns.com/foaf/0.1/"/>
    <owl:imports rdf:resource="http://purl.org/dc/terms/"/>
    <owl:imports rdf:resource="http://www.w3.org/ns/org#"/>
    <owl:imports rdf:resource="http://www.w3.org/2004/02/skos/core"/>
    <owl:imports rdf:resource="http://data.europa.eu/nuts"/>
    <owl:imports rdf:resource="http://publications.europa.eu/resource/authority/"/>
    <owl:imports rdf:resource="http://www.w3.org/2006/time"/>
    <owl:imports rdf:resource="http://www.w3.org/ns/locn"/>
    <owl:imports rdf:resource="https://data.europa.eu/m8g/"/>
    <owl:imports rdf:resource="http://data.europa.eu/m8g/"/>
    <owl:imports rdf:resource="http://www.opengis.net/ont/geosparql"/>
    <owl:imports rdf:resource="http://www.w3.org/ns/person"/>
    <owl:imports rdf:resource="http://www.w3.org/ns/adms"/>
    <owl:imports rdf:resource="http://purl.org/ontology/bibo/"/>
    <owl:imports rdf:resource="http://www.w3.org/ns/dcat"/>
    <owl:imports rdf:resource="http://www.w3.org/ns/odrl/2/"/>
    <owl:imports rdf:resource="http://data.europa.eu/r5r/"/>
    <owl:imports rdf:resource="http://www.w3.org/ns/prov#"/>
    <owl:imports rdf:resource="http://spdx.org/rdf/terms#"/>
    <owl:imports rdf:resource="http://purl.org/dc/dcmitype/"/>
    <owl:imports rdf:resource="https://w3id.org/dpv#"/>
    <owl:imports rdf:resource="http://www.w3.org/2006/vcard/ns"/>
    <dcterms:title xml:lang="en">ePO Core core</dcterms:title>
    <rdfs:label xml:lang="en">This artefact provides the definitions for the eProcurement Ontology Core.         This artefact excludes the restrictions.         The eProcurement Ontology describes objects and concepts, with definitions, attributes and relationships which are present within the European public procurement domain.         The provision of these concepts provides the basis for a common understanding of the domain for all stakeholders ensuring the quality of data exchange and transparency.</rdfs:label>
    <dcterms:description xml:lang="en">This artefact provides the definitions for the eProcurement Ontology Core.         This artefact excludes the restrictions.         The eProcurement Ontology describes objects and concepts, with definitions, attributes and relationships which are present within the European public procurement domain.         The provision of these concepts provides the basis for a common understanding of the domain for all stakeholders ensuring the quality of data exchange and transparency.</dcterms:description>
    <dcterms:publisher>http://publications.europa.eu/resource/authority/corporate-body/PUBL</dcterms:publisher>
    <rdfs:comment>This version is automatically generated from dcat_ap_lu_CM.xml on 2025-07-30</rdfs:comment>
    <rdfs:seeAlso rdf:resource="https://github.com/eprocurementontology/eprocurementontology"/>
    <rdfs:seeAlso rdf:resource="https://joinup.ec.europa.eu/collection/eprocurement/solution/eprocurement-ontology/about"/>
    <rdfs:seeAlso rdf:resource="https://op.europa.eu/en/web/eu-vocabularies/e-procurement"/>
    <rdfs:seeAlso rdf:resource="https://docs.ted.europa.eu/EPO/latest/index.html"/>
    <dcterms:issued rdf:datatype="http://www.w3.org/2001/XMLSchema#date">2025-07-30</dcterms:issued>
    <dcterms:created rdf:datatype="http://www.w3.org/2001/XMLSchema#date">2025-07-30</dcterms:created>
    <owl:versionInfo>3.1.0</owl:versionInfo>
    <owl:incompatibleWith>2.1.0</owl:incompatibleWith>
    <owl:versionIRI rdf:resource="http://data.europa.eu/a4g/ontology#core-3.1.0"/>
    <owl:priorVersion>http://data.europa.eu/a4g/ontology#core-3.0.1</owl:priorVersion>
    <vann:preferredNamespaceUri>http://data.europa.eu/a4g/ontology#</vann:preferredNamespaceUri>
    <vann:preferredNamespacePrefix>epo</vann:preferredNamespacePrefix>
    <dcterms:license>The Commission’s reuse policy is implemented by Commission Decision2011/833/EU of 12 December 2011 on the reuse of Commission documents          (OJ L 330,14.12.2011, p. 39 – https://eur-lex.europa.eu/eli/dec/2011/833/oj). Unlessotherwise noted, the reuse of this document is authorised under the          CreativeCommons Attribution 4.0 International (CC BY 4.0) licence (https://creativecommons.org/licenses/by/4.0/).This means that reuse is allowed, provided          that appropriate credit is given and any changes are indicated.</dcterms:license>
  </rdf:Description>
  <rdf:Description rdf:about="http://purl.org/dc/terms/accessRights">
    <rdf:type rdf:resource="http://www.w3.org/2002/07/owl#ObjectProperty"/>
    <skos:prefLabel xml:lang="en">access Rights</skos:prefLabel>
    <skos:definition xml:lang="en">Information that indicates whether the Dataset is publicly accessible, has access restrictions or is not public. Usage note: DCAT-AP-LU places additional restrictions on the vocabularies recommended in DCAT-AP. See section 10. Controlled Vocabularies for details.</skos:definition>
  </rdf:Description>
  <rdf:Description rdf:about="http://purl.org/dc/terms/conformsTo">
    <rdf:type rdf:resource="http://www.w3.org/2002/07/owl#ObjectProperty"/>
    <skos:prefLabel xml:lang="en">conforms To</skos:prefLabel>
    <skos:definition xml:lang="en">An implementing rule or other specification.</skos:definition>
  </rdf:Description>
  <rdf:Description rdf:about="http://www.w3.org/ns/dcat#DatasetSeries">
    <rdf:type rdf:resource="http://www.w3.org/2002/07/owl#Class"/>
    <skos:prefLabel xml:lang="en">Dataset Series</skos:prefLabel>
    <skos:definition xml:lang="en">A collection of datasets that are published separately, but share some characteristics that group them. Usage Note It is recommended to avoid Dataset Series without a dataset in the collection. Therefore at least one Dataset should refer to a Dataset Series using the property in series (dcat:inSeries).</skos:definition>
  </rdf:Description>
  <rdf:Description rdf:about="http://www.w3.org/2006/vcard/ns#Kind">
    <rdf:type rdf:resource="http://www.w3.org/2002/07/owl#Class"/>
    <skos:prefLabel xml:lang="en">Kind</skos:prefLabel>
    <skos:definition xml:lang="en">A description following the vCard specification, e.g. to provide telephone number and e-mail address for a contact point.</skos:definition>
  </rdf:Description>
  <rdf:Description rdf:about="http://purl.org/dc/terms/type">
    <rdf:type rdf:resource="http://www.w3.org/2002/07/owl#ObjectProperty"/>
    <skos:prefLabel xml:lang="en">type</skos:prefLabel>
    <skos:definition xml:lang="en">A type of the Dataset. Usage:DCAT-AP-LU extends the recommendations for controlled vocabularies for this properties provided by DCAT-AP. A type of licence, e.g. indicating 'public domain' or 'royalties required'.</skos:definition>
  </rdf:Description>
  <rdf:Description rdf:about="http://purl.org/dc/terms/Frequency">
    <rdf:type rdf:resource="http://www.w3.org/2002/07/owl#Class"/>
    <skos:prefLabel xml:lang="en">Frequency</skos:prefLabel>
    <skos:definition xml:lang="en">A rate at which something recurs, e.g. the publication of a Dataset.</skos:definition>
  </rdf:Description>
  <rdf:Description rdf:about="http://www.w3.org/ns/dcat#distribution">
    <rdf:type rdf:resource="http://www.w3.org/2002/07/owl#ObjectProperty"/>
    <skos:prefLabel xml:lang="en">distribution</skos:prefLabel>
    <skos:definition xml:lang="en">An available Distribution for the Dataset.</skos:definition>
  </rdf:Description>
  <rdf:Description rdf:about="http://purl.org/dc/terms/publisher">
    <rdf:type rdf:resource="http://www.w3.org/2002/07/owl#ObjectProperty"/>
    <skos:prefLabel xml:lang="en">publisher</skos:prefLabel>
    <skos:definition xml:lang="en">An entity (organisation) responsible for making the Dataset available. Usage: DCAT-AP-LU provides additional usage guidance regarding vocabularies for publishers An entity (organisation) responsible for making the Dataset available. Usage note: DCAT-AP-LU provides additional usage guidance regarding vocabularies for publishers</skos:definition>
  </rdf:Description>
  <rdf:Description rdf:about="http://purl.org/dc/terms/LinguisticSystem">
    <rdf:type rdf:resource="http://www.w3.org/2002/07/owl#Class"/>
    <skos:prefLabel xml:lang="en">Linguistic System</skos:prefLabel>
  </rdf:Description>
  <rdf:Description rdf:about="http://www.w3.org/ns/prov#Attribution">
    <rdf:type rdf:resource="http://www.w3.org/2002/07/owl#Class"/>
    <skos:prefLabel xml:lang="en">Attribution</skos:prefLabel>
    <skos:definition xml:lang="en">Attribution is the ascribing of an entity to an agent.</skos:definition>
  </rdf:Description>
  <rdf:Description rdf:about="http://spdx.org/rdf/terms#checksum">
    <rdf:type rdf:resource="http://www.w3.org/2002/07/owl#ObjectProperty"/>
    <skos:prefLabel xml:lang="en">checksum</skos:prefLabel>
    <skos:definition xml:lang="en">A mechanism that can be used to verify that the contents of a distribution have not changed.</skos:definition>
  </rdf:Description>
  <rdf:Description rdf:about="http://www.w3.org/ns/dcat#packageFormat">
    <rdf:type rdf:resource="http://www.w3.org/2002/07/owl#ObjectProperty"/>
    <skos:prefLabel xml:lang="en">package Format</skos:prefLabel>
    <skos:definition xml:lang="en">The format of the file in which one or more data files are grouped together, e.g. to enable a set of related files to be downloaded together.</skos:definition>
  </rdf:Description>
  <rdf:Description rdf:about="http://purl.org/dc/terms/rights">
    <rdf:type rdf:resource="http://www.w3.org/2002/07/owl#ObjectProperty"/>
    <skos:prefLabel xml:lang="en">rights</skos:prefLabel>
    <skos:definition xml:lang="en">A statement that specifies rights associated with the Distribution.</skos:definition>
  </rdf:Description>
  <rdf:Description rdf:about="http://www.w3.org/ns/adms#identifier">
    <rdf:type rdf:resource="http://www.w3.org/2002/07/owl#ObjectProperty"/>
    <skos:prefLabel xml:lang="en">identifier</skos:prefLabel>
    <skos:definition xml:lang="en">A secondary identifier of the Dataset</skos:definition>
  </rdf:Description>
  <rdf:Description rdf:about="http://purl.org/dc/terms/provenance">
    <rdf:type rdf:resource="http://www.w3.org/2002/07/owl#ObjectProperty"/>
    <skos:prefLabel xml:lang="en">provenance</skos:prefLabel>
    <skos:definition xml:lang="en">A statement about the lineage of a Dataset. DCAT-AP-LU recommends the use of this property. Refer to usage guidance for details.</skos:definition>
  </rdf:Description>
  <rdf:Description rdf:about="http://www.w3.org/ns/adms#versionNotes">
    <rdf:type rdf:resource="http://www.w3.org/2002/07/owl#ObjectProperty"/>
    <skos:prefLabel xml:lang="en">version Notes</skos:prefLabel>
    <skos:definition xml:lang="en">A description of the differences between this version and a previous version of the Dataset. (dcat:Dataset)</skos:definition>
  </rdf:Description>
  <rdf:Description rdf:about="http://purl.org/dc/terms/modified">
    <rdf:type rdf:resource="http://www.w3.org/1999/02/22-rdf-syntax-ns#Property"/>
    <skos:prefLabel xml:lang="en">modified</skos:prefLabel>
    <skos:definition xml:lang="en">The most recent date on which the Dataset was changed or modified. (dcat:Dataset) The most recent date on which the Dataset Series was changed or modified. (dcat:DatasetSeries) The most recent date on which the Distribution was changed or modified. (dcat:Distribution)</skos:definition>
  </rdf:Description>
  <rdf:Description rdf:about="http://www.w3.org/ns/dcat#DataService">
    <rdf:type rdf:resource="http://www.w3.org/2002/07/owl#Class"/>
    <skos:prefLabel xml:lang="en">Data Service</skos:prefLabel>
    <skos:definition xml:lang="en">A collection of operations that provides access to one or more datasets or data processing functions.</skos:definition>
  </rdf:Description>
  <rdf:Description rdf:about="http://www.w3.org/ns/dcat#mediaType">
    <rdf:type rdf:resource="http://www.w3.org/2002/07/owl#ObjectProperty"/>
    <skos:prefLabel xml:lang="en">media Type</skos:prefLabel>
    <skos:definition xml:lang="en">The media type of the Distribution as defined in the official register of media types managed by IANA. Usage note: DCAT-AP-LU provides additional usage guidance for this property.</skos:definition>
  </rdf:Description>
  <rdf:Description rdf:about="http://purl.org/dc/terms/format">
    <rdf:type rdf:resource="http://www.w3.org/2002/07/owl#ObjectProperty"/>
    <skos:prefLabel xml:lang="en">format</skos:prefLabel>
    <skos:definition xml:lang="en">The file format of the Distribution.</skos:definition>
  </rdf:Description>
  <rdf:Description rdf:about="http://purl.org/dc/terms/MediaTypeOrExtent">
    <rdf:type rdf:resource="http://www.w3.org/2002/07/owl#Class"/>
    <skos:prefLabel xml:lang="en">Media Type Or Extent</skos:prefLabel>
    <skos:definition xml:lang="en">A media type or dataset distribution.</skos:definition>
  </rdf:Description>
  <rdf:Description rdf:about="http://purl.org/dc/terms/PeriodOfTime">
    <rdf:type rdf:resource="http://www.w3.org/2002/07/owl#Class"/>
    <skos:prefLabel xml:lang="en">Period Of Time</skos:prefLabel>
  </rdf:Description>
  <rdf:Description rdf:about="http://www.w3.org/ns/dcat#byteSize">
    <rdf:type rdf:resource="http://www.w3.org/2002/07/owl#DatatypeProperty"/>
    <skos:prefLabel xml:lang="en">byte Size</skos:prefLabel>
    <skos:definition xml:lang="en">The size of a Distribution in bytes. (dcat:Distribution)</skos:definition>
  </rdf:Description>
  <rdf:Description rdf:about="http://www.w3.org/ns/dcat#qualifiedRelation">
    <rdf:type rdf:resource="http://www.w3.org/2002/07/owl#ObjectProperty"/>
    <skos:prefLabel xml:lang="en">qualified Relation</skos:prefLabel>
    <skos:definition xml:lang="en">A description of a relationship with another resource</skos:definition>
  </rdf:Description>
  <rdf:Description rdf:about="http://purl.org/dc/terms/isReferencedBy">
    <rdf:type rdf:resource="http://www.w3.org/1999/02/22-rdf-syntax-ns#Property"/>
    <skos:prefLabel xml:lang="en">is Referenced By</skos:prefLabel>
    <skos:definition xml:lang="en">A related resource, such as a publication, that references, cites, or otherwise points to the dataset. (dcat:Dataset)</skos:definition>
  </rdf:Description>
  <rdf:Description rdf:about="http://www.w3.org/ns/dcat#theme">
    <rdf:type rdf:resource="http://www.w3.org/2002/07/owl#ObjectProperty"/>
    <skos:prefLabel xml:lang="en">theme</skos:prefLabel>
    <skos:definition xml:lang="en">A category of the Dataset. Usage: A Dataset may be associated with multiple themes. Note: the theme is an URI not URL therefore, it may not properly resolve in the web browser even though it properly resolves through the API.</skos:definition>
  </rdf:Description>
  <rdf:Description rdf:about="http://purl.org/dc/terms/title">
    <rdf:type rdf:resource="http://www.w3.org/2002/07/owl#ObjectProperty"/>
    <skos:prefLabel xml:lang="en">title</skos:prefLabel>
    <skos:definition xml:lang="en">A name given to the Dataset (dcat:Dataset) A name given to the Dataset Series. (dcat:DatasetSeries) A name given to the Distribution. (dcat:Distribution)</skos:definition>
  </rdf:Description>
  <rdf:Description rdf:about="http://purl.org/dc/terms/RightsStatement">
    <rdf:type rdf:resource="http://www.w3.org/2002/07/owl#Class"/>
    <skos:prefLabel xml:lang="en">Rights Statement</skos:prefLabel>
    <skos:definition xml:lang="en">A statement about the intellectual property rights (IPR) held in or over a resource, a legal document giving official permission to do something with a resource, or a statement about access rights.</skos:definition>
  </rdf:Description>
  <rdf:Description rdf:about="http://spdx.org/rdf/terms#Checksum">
    <rdf:type rdf:resource="http://www.w3.org/2002/07/owl#Class"/>
    <skos:prefLabel xml:lang="en">Checksum</skos:prefLabel>
    <skos:definition xml:lang="en">A Checksum is value that allows the contents of a file to be authenticated. Even small changes to the content of the file will change its checksum. This class allows the results of a variety of checksum and cryptographic message digest algorithms to be represented.</skos:definition>
  </rdf:Description>
  <rdf:Description rdf:about="http://www.w3.org/ns/dcat#Dataset">
    <rdf:type rdf:resource="http://www.w3.org/2002/07/owl#Class"/>
    <skos:prefLabel xml:lang="en">Dataset</skos:prefLabel>
    <rdfs:subClassOf rdf:resource="http://www.w3.org/ns/dcat#Resource"/>
  </rdf:Description>
  <rdf:Description rdf:about="http://xmlns.com/foaf/0.1/Document">
    <rdf:type rdf:resource="http://www.w3.org/2002/07/owl#Class"/>
    <skos:prefLabel xml:lang="en">Document</skos:prefLabel>
  </rdf:Description>
  <rdf:Description rdf:about="http://www.w3.org/ns/prov#Activity">
    <rdf:type rdf:resource="http://www.w3.org/2002/07/owl#Class"/>
    <skos:prefLabel xml:lang="en">Activity</skos:prefLabel>
    <skos:definition xml:lang="en">An activity is something that occurs over a period of time and acts upon or with entities; it may include consuming, processing, transforming, modifying, relocating, using, or generating entities.</skos:definition>
  </rdf:Description>
  <rdf:Description rdf:about="http://purl.org/dc/terms/isVersionOf">
    <rdf:type rdf:resource="http://www.w3.org/2002/07/owl#ObjectProperty"/>
    <skos:prefLabel xml:lang="en">is Version Of</skos:prefLabel>
  </rdf:Description>
  <rdf:Description rdf:about="https://w3id.org/dpv#hasData">
    <rdf:type rdf:resource="http://www.w3.org/2002/07/owl#ObjectProperty"/>
    <skos:prefLabel xml:lang="en">has Data</skos:prefLabel>
    <skos:definition xml:lang="en">The type(s) of data protection, as defined in the context of the DGA, that applies to the dataset. Usage:A list of accepted types, based on the Data Privacy Vocabulary</skos:definition>
  </rdf:Description>
  <rdf:Description rdf:about="http://purl.org/dc/terms/spatial">
    <rdf:type rdf:resource="http://www.w3.org/2002/07/owl#ObjectProperty"/>
    <skos:prefLabel xml:lang="en">spatial</skos:prefLabel>
    <skos:definition xml:lang="en">A geographic region that is covered by the Dataset. A geographic region that is covered by the Dataset Series</skos:definition>
  </rdf:Description>
  <rdf:Description rdf:about="http://www.w3.org/ns/dcat#Relationship">
    <rdf:type rdf:resource="http://www.w3.org/2002/07/owl#Class"/>
    <skos:prefLabel xml:lang="en">Relationship</skos:prefLabel>
  </rdf:Description>
  <rdf:Description rdf:about="http://www.w3.org/ns/dcat#accessService">
    <rdf:type rdf:resource="http://www.w3.org/2002/07/owl#ObjectProperty"/>
    <skos:prefLabel xml:lang="en">access Service</skos:prefLabel>
    <skos:definition xml:lang="en">A data service that gives access to the distribution of the dataset.</skos:definition>
  </rdf:Description>
  <rdf:Description rdf:about="http://www.w3.org/ns/locn#Geometry">
    <rdf:type rdf:resource="http://www.w3.org/2002/07/owl#Class"/>
    <skos:prefLabel xml:lang="en">Geometry</skos:prefLabel>
    <skos:definition xml:lang="en">The Geometry class provides the means to identify a Location as a point, line, polygon, etc. expressed using coordinates in some coordinate reference System.</skos:definition>
  </rdf:Description>
  <rdf:Description rdf:about="http://www.w3.org/ns/dcat#inSeries">
    <rdf:type rdf:resource="http://www.w3.org/2002/07/owl#ObjectProperty"/>
    <skos:prefLabel xml:lang="en">in Series</skos:prefLabel>
    <skos:definition xml:lang="en">A dataset series of which the dataset is part. Usage Note: DCAT-AP-LU recommends the use of DatasetSeries, with additional guidance provided</skos:definition>
  </rdf:Description>
  <rdf:Description rdf:about="http://www.w3.org/ns/dcat#compressFormat">
    <rdf:type rdf:resource="http://www.w3.org/2002/07/owl#ObjectProperty"/>
    <skos:prefLabel xml:lang="en">compress Format</skos:prefLabel>
    <skos:definition xml:lang="en">compressed form, e.g. to reduce the size of the downloadable file. Usage Note: It SHOULD be expressed using a media type as defined in the official register of media types managed by IANA.</skos:definition>
  </rdf:Description>
  <rdf:Description rdf:about="http://www.w3.org/ns/dcat#bbox">
    <rdf:type rdf:resource="http://www.w3.org/2002/07/owl#ObjectProperty"/>
    <skos:prefLabel xml:lang="en">bbox</skos:prefLabel>
  </rdf:Description>
  <rdf:Description rdf:about="http://www.w3.org/2004/02/skos/core#notation">
    <rdf:type rdf:resource="http://www.w3.org/2002/07/owl#ObjectProperty"/>
    <skos:prefLabel xml:lang="en">notation</skos:prefLabel>
    <skos:definition xml:lang="en">The literal identifying an entity, like a person or an object. (adms:Identifier)</skos:definition>
  </rdf:Description>
  <rdf:Description rdf:about="http://www.w3.org/ns/dcat#Resource">
    <rdf:type rdf:resource="http://www.w3.org/2002/07/owl#Class"/>
    <skos:prefLabel xml:lang="en">Resource</skos:prefLabel>
    <skos:definition xml:lang="en">Resource published or curated by a single agent.</skos:definition>
  </rdf:Description>
  <rdf:Description rdf:about="http://www.w3.org/ns/adms#status">
    <rdf:type rdf:resource="http://www.w3.org/2002/07/owl#ObjectProperty"/>
    <skos:prefLabel xml:lang="en">status</skos:prefLabel>
  </rdf:Description>
  <rdf:Description rdf:about="http://www.w3.org/ns/odrl/2/hasPolicy">
    <rdf:type rdf:resource="http://www.w3.org/2002/07/owl#ObjectProperty"/>
    <skos:prefLabel xml:lang="en">has Policy</skos:prefLabel>
    <skos:definition xml:lang="en">The policy expressing the rights associated with the distribution if using the [ODRL] vocabulary. DCAT-AP-LU provides additional usage guidance on the use of this property for expressing data use restrictions.</skos:definition>
  </rdf:Description>
  <rdf:Description rdf:about="https://w3id.org/dpv#Data">
    <rdf:type rdf:resource="http://www.w3.org/2002/07/owl#Class"/>
    <skos:prefLabel xml:lang="en">Data</skos:prefLabel>
    <skos:definition xml:lang="en">A broad concept representing 'data' or 'information'</skos:definition>
    <rdfs:subClassOf rdf:resource="http://www.w3.org/2004/02/skos/core#Concept"/>
  </rdf:Description>
  <rdf:Description rdf:about="http://www.w3.org/ns/dcat#downloadURL">
    <rdf:type rdf:resource="http://www.w3.org/1999/02/22-rdf-syntax-ns#Property"/>
    <skos:prefLabel xml:lang="en">download URL</skos:prefLabel>
    <skos:definition xml:lang="en">A URL that is a direct link to a downloadable file in a given format. (dcat:Distribution)</skos:definition>
  </rdf:Description>
  <rdf:Description rdf:about="http://purl.org/dc/terms/language">
    <rdf:type rdf:resource="http://www.w3.org/2002/07/owl#ObjectProperty"/>
    <skos:prefLabel xml:lang="en">language</skos:prefLabel>
    <skos:definition xml:lang="en">A language of the Dataset. A language used in the Distribution.</skos:definition>
  </rdf:Description>
  <rdf:Description rdf:about="http://purl.org/dc/terms/relation">
    <rdf:type rdf:resource="http://www.w3.org/1999/02/22-rdf-syntax-ns#Property"/>
    <skos:prefLabel xml:lang="en">relation</skos:prefLabel>
    <skos:definition xml:lang="en">A related resource. (dcat:Dataset)</skos:definition>
  </rdf:Description>
  <rdf:Description rdf:about="http://www.w3.org/ns/dcat#temporalResolution">
    <rdf:type rdf:resource="http://www.w3.org/1999/02/22-rdf-syntax-ns#Property"/>
    <skos:prefLabel xml:lang="en">temporal Resolution</skos:prefLabel>
    <skos:definition xml:lang="en">The minimum time period resolvable in the dataset. (dcat:Dataset) The minimum time period resolvable in the dataset distribution. (dcat:Distribution)</skos:definition>
  </rdf:Description>
  <rdf:Description rdf:about="http://purl.org/dc/terms/issued">
    <rdf:type rdf:resource="http://www.w3.org/1999/02/22-rdf-syntax-ns#Property"/>
    <skos:prefLabel xml:lang="en">issued</skos:prefLabel>
    <skos:definition xml:lang="en">The date of formal issuance (e.g., publication) of the Dataset. (dcat:Dataset) The date of formal issuance (e.g., publication) of the Dataset Series. (dcat:DatasetSeries) The date of formal issuance (e.g., publication) of the Distribution. (dcat:Distribution)</skos:definition>
  </rdf:Description>
  <rdf:Description rdf:about="http://purl.org/dc/terms/source">
    <rdf:type rdf:resource="http://www.w3.org/2002/07/owl#ObjectProperty"/>
    <skos:prefLabel xml:lang="en">source</skos:prefLabel>
    <skos:definition xml:lang="en">A related Dataset from which the described Dataset is derived.</skos:definition>
  </rdf:Description>
  <rdf:Description rdf:about="http://www.w3.org/ns/dcat#keyword">
    <rdf:type rdf:resource="http://www.w3.org/2002/07/owl#ObjectProperty"/>
    <skos:prefLabel xml:lang="en">keyword</skos:prefLabel>
    <skos:definition xml:lang="en">A keyword or tag describing the Dataset. (dcat:Dataset)</skos:definition>
  </rdf:Description>
  <rdf:Description rdf:about="http://xmlns.com/foaf/0.1/name">
    <rdf:type rdf:resource="http://www.w3.org/2002/07/owl#ObjectProperty"/>
    <skos:prefLabel xml:lang="en">name</skos:prefLabel>
  </rdf:Description>
  <rdf:Description rdf:about="http://purl.org/dc/terms/identifier">
    <rdf:type rdf:resource="http://www.w3.org/2002/07/owl#ObjectProperty"/>
    <skos:prefLabel xml:lang="en">identifier</skos:prefLabel>
    <skos:definition xml:lang="en">The main identifier for the Dataset, e.g. the URI or other unique identifier in the context of the Catalogue. Usage Note: The use of persistent dereferenceable URIs is mandatory in this profile. (dcat:Dataset)</skos:definition>
  </rdf:Description>
  <rdf:Description rdf:about="http://purl.org/dc/terms/accrualPeriodicity">
    <rdf:type rdf:resource="http://www.w3.org/2002/07/owl#ObjectProperty"/>
    <skos:prefLabel xml:lang="en">accrual Periodicity</skos:prefLabel>
    <skos:definition xml:lang="en">The frequency at which the Dataset is updated. The frequency at which the Dataset series is updated.</skos:definition>
  </rdf:Description>
  <rdf:Description rdf:about="http://data.europa.eu/r5r/applicablelegislation">
    <rdf:type rdf:resource="http://www.w3.org/2002/07/owl#ObjectProperty"/>
    <skos:prefLabel xml:lang="en">applicablelegislation</skos:prefLabel>
    <skos:definition xml:lang="en">The legislation that mandates the creation or management of the Dataset. Usage: DCAT-AP-LU provides additional usage guidance for this property in the DGA context. The legislation that mandates the creation or management of the Dataset Series.</skos:definition>
  </rdf:Description>
  <rdf:Description rdf:about="http://xmlns.com/foaf/0.1/Agent">
    <rdf:type rdf:resource="http://www.w3.org/2002/07/owl#Class"/>
    <skos:prefLabel xml:lang="en">Agent</skos:prefLabel>
  </rdf:Description>
  <rdf:Description rdf:about="http://data.europa.eu/eli/ontology#LegalResource">
    <rdf:type rdf:resource="http://www.w3.org/2002/07/owl#Class"/>
    <skos:prefLabel xml:lang="en">Legal Resource</skos:prefLabel>
    <skos:definition xml:lang="en">This class represents the legislation, policy or policies that lie behind the Rules that govern the service. Usage Note The definition and properties of the Legal Resource class are aligned with the ontology included in "Council conclusions inviting the introduction of the European Legislation Identifier (ELI)". For describing the attributes of a Legal Resource (labels, preferred labels, alternative labels, definition, etc.) we refer to the ELI ontology. In this data specification the use is restricted to instances of this class that follow the ELI URI guidelines</skos:definition>
  </rdf:Description>
  <rdf:Description rdf:about="http://data.europa.eu/r5r/availability">
    <rdf:type rdf:resource="http://www.w3.org/2002/07/owl#ObjectProperty"/>
    <skos:prefLabel xml:lang="en">availability</skos:prefLabel>
    <skos:definition xml:lang="en">An indication how long it is planned to keep the Distribution of the Dataset available.</skos:definition>
  </rdf:Description>
  <rdf:Description rdf:about="http://purl.org/dc/terms/temporal">
    <rdf:type rdf:resource="http://www.w3.org/2002/07/owl#ObjectProperty"/>
    <skos:prefLabel xml:lang="en">temporal</skos:prefLabel>
    <skos:definition xml:lang="en">A temporal period that the Dataset covers.</skos:definition>
  </rdf:Description>
  <rdf:Description rdf:about="http://www.w3.org/2006/time#hasEnd">
    <rdf:type rdf:resource="http://www.w3.org/1999/02/22-rdf-syntax-ns#Property"/>
    <skos:prefLabel xml:lang="en">has End</skos:prefLabel>
  </rdf:Description>
  <rdf:Description rdf:about="http://www.w3.org/ns/dcat#landingPage">
    <rdf:type rdf:resource="http://www.w3.org/2002/07/owl#ObjectProperty"/>
    <skos:prefLabel xml:lang="en">landing Page</skos:prefLabel>
    <skos:definition xml:lang="en">A web page that provides access to the Dataset, its Distributions and/or additional information.</skos:definition>
  </rdf:Description>
  <rdf:Description rdf:about="http://www.w3.org/ns/prov#qualifiedAttribution">
    <rdf:type rdf:resource="http://www.w3.org/2002/07/owl#ObjectProperty"/>
    <skos:prefLabel xml:lang="en">qualified Attribution</skos:prefLabel>
    <skos:definition xml:lang="en">An Agent having some form of responsibility for the resource.</skos:definition>
  </rdf:Description>
  <rdf:Description rdf:about="http://www.w3.org/ns/prov#qualifiedRelation">
    <rdf:type rdf:resource="http://www.w3.org/2002/07/owl#ObjectProperty"/>
    <skos:prefLabel xml:lang="en">qualified Relation</skos:prefLabel>
    <skos:definition xml:lang="en">A description of a relationship with another resource.</skos:definition>
  </rdf:Description>
  <rdf:Description rdf:about="http://www.w3.org/2004/02/skos/core#inScheme">
    <rdf:type rdf:resource="http://www.w3.org/2002/07/owl#ObjectProperty"/>
    <skos:prefLabel xml:lang="en">in Scheme</skos:prefLabel>
  </rdf:Description>
  <rdf:Description rdf:about="http://www.w3.org/2002/07/owl#versionInfo">
    <rdf:type rdf:resource="http://www.w3.org/2002/07/owl#ObjectProperty"/>
    <skos:prefLabel xml:lang="en">version Info</skos:prefLabel>
  </rdf:Description>
  <rdf:Description rdf:about="http://www.w3.org/ns/dcat#spatialResolutionInMeters">
    <rdf:type rdf:resource="http://www.w3.org/2002/07/owl#DatatypeProperty"/>
    <skos:prefLabel xml:lang="en">spatial Resolution In Meters</skos:prefLabel>
    <skos:definition xml:lang="en">The minimum spatial separation resolvable in a dataset, measured in meters. (dcat:Dataset) The minimum spatial separation resolvable in a dataset distribution, measured in meters. (dcat:Distribution)</skos:definition>
  </rdf:Description>
  <rdf:Description rdf:about="http://xmlns.com/foaf/0.1/page">
    <rdf:type rdf:resource="http://www.w3.org/2002/07/owl#ObjectProperty"/>
    <skos:prefLabel xml:lang="en">page</skos:prefLabel>
    <skos:definition xml:lang="en">A page or document about this Dataset. A page or document about this Distribution.</skos:definition>
  </rdf:Description>
  <rdf:Description rdf:about="http://www.w3.org/2006/time#hasBeginning">
    <rdf:type rdf:resource="http://www.w3.org/1999/02/22-rdf-syntax-ns#Property"/>
    <skos:prefLabel xml:lang="en">has Beginning</skos:prefLabel>
  </rdf:Description>
  <rdf:Description rdf:about="http://www.w3.org/ns/locn#geometry">
    <rdf:type rdf:resource="http://www.w3.org/2002/07/owl#ObjectProperty"/>
    <skos:prefLabel xml:lang="en">geometry</skos:prefLabel>
  </rdf:Description>
  <rdf:Description rdf:about="http://purl.org/dc/terms/Location">
    <rdf:type rdf:resource="http://www.w3.org/2002/07/owl#Class"/>
    <skos:prefLabel xml:lang="en">Location</skos:prefLabel>
    <skos:definition xml:lang="en">A temporal period that the Dataset covers.</skos:definition>
  </rdf:Description>
  <rdf:Description rdf:about="http://www.w3.org/ns/dcat#contactPoint">
    <rdf:type rdf:resource="http://www.w3.org/2002/07/owl#ObjectProperty"/>
    <skos:prefLabel xml:lang="en">contact Point</skos:prefLabel>
    <skos:definition xml:lang="en">Contact information that can be used for sending comments about the Dataset. Contact information that can be used for sending comments about the DatasetSeries.</skos:definition>
  </rdf:Description>
  <rdf:Description rdf:about="http://purl.org/dc/terms/description">
    <rdf:type rdf:resource="http://www.w3.org/2002/07/owl#ObjectProperty"/>
    <skos:prefLabel xml:lang="en">description</skos:prefLabel>
    <skos:definition xml:lang="en">A free-text account of the Dataset. (dcat:Dataset) A free-text account of the Dataset Series. (dcat:DatasetSeries) A free-text account of the Distribution. (dcat:Distribution)</skos:definition>
  </rdf:Description>
  <rdf:Description rdf:about="http://www.w3.org/ns/dcat#startDate">
    <rdf:type rdf:resource="http://www.w3.org/1999/02/22-rdf-syntax-ns#Property"/>
    <skos:prefLabel xml:lang="en">start Date</skos:prefLabel>
  </rdf:Description>
  <rdf:Description rdf:about="http://www.w3.org/ns/dcat#centroid">
    <rdf:type rdf:resource="http://www.w3.org/2002/07/owl#ObjectProperty"/>
    <skos:prefLabel xml:lang="en">centroid</skos:prefLabel>
  </rdf:Description>
  <rdf:Description rdf:about="http://purl.org/dc/terms/hasVersion">
    <rdf:type rdf:resource="http://www.w3.org/2002/07/owl#ObjectProperty"/>
    <skos:prefLabel xml:lang="en">has Version</skos:prefLabel>
    <skos:definition xml:lang="en">A related Dataset that is a version, edition, or adaptation of the described Dataset.</skos:definition>
  </rdf:Description>
  <rdf:Description rdf:about="http://purl.org/dc/terms/ProvenanceStatement">
    <rdf:type rdf:resource="http://www.w3.org/2002/07/owl#Class"/>
    <skos:prefLabel xml:lang="en">Provenance Statement</skos:prefLabel>
    <skos:definition xml:lang="en">Any changes in ownership and custody of a resource since its creation that are significant for its authenticity, integrity, and interpretation.</skos:definition>
  </rdf:Description>
  <rdf:Description rdf:about="http://purl.org/dc/terms/Standard">
    <rdf:type rdf:resource="http://www.w3.org/2002/07/owl#Class"/>
    <skos:prefLabel xml:lang="en">Standard</skos:prefLabel>
  </rdf:Description>
  <rdf:Description rdf:about="http://www.w3.org/2004/02/skos/core#Concept">
    <rdf:type rdf:resource="http://www.w3.org/2002/07/owl#Class"/>
    <skos:prefLabel xml:lang="en">Concept</skos:prefLabel>
  </rdf:Description>
  <rdf:Description rdf:about="http://purl.org/dc/terms/creator">
    <rdf:type rdf:resource="http://www.w3.org/2002/07/owl#ObjectProperty"/>
    <skos:prefLabel xml:lang="en">creator</skos:prefLabel>
    <skos:definition xml:lang="en">An entity responsible for producing the dataset.</skos:definition>
  </rdf:Description>
  <rdf:Description rdf:about="http://www.w3.org/ns/dcat#accessURL">
    <rdf:type rdf:resource="http://www.w3.org/1999/02/22-rdf-syntax-ns#Property"/>
    <skos:prefLabel xml:lang="en">access URL</skos:prefLabel>
    <skos:definition xml:lang="en">A URL that gives access to a Distribution of the Dataset. (dcat:Distribution)</skos:definition>
  </rdf:Description>
  <rdf:Description rdf:about="http://purl.org/dc/terms/MediaType">
    <rdf:type rdf:resource="http://www.w3.org/2002/07/owl#Class"/>
    <skos:prefLabel xml:lang="en">Media Type</skos:prefLabel>
    <skos:definition xml:lang="en">A file format or physical medium.</skos:definition>
  </rdf:Description>
  <rdf:Description rdf:about="http://www.w3.org/ns/dcat#endDate">
    <rdf:type rdf:resource="http://www.w3.org/1999/02/22-rdf-syntax-ns#Property"/>
    <skos:prefLabel xml:lang="en">end Date</skos:prefLabel>
  </rdf:Description>
  <rdf:Description rdf:about="http://www.w3.org/ns/dcat#Distribution">
    <rdf:type rdf:resource="http://www.w3.org/2002/07/owl#Class"/>
    <skos:prefLabel xml:lang="en">Distribution</skos:prefLabel>
    <skos:definition xml:lang="en">A physical embodiment of the Dataset in a particular format.</skos:definition>
  </rdf:Description>
  <rdf:Description rdf:about="http://www.w3.org/ns/prov#wasGeneratedBy">
    <rdf:type rdf:resource="http://www.w3.org/2002/07/owl#ObjectProperty"/>
    <skos:prefLabel xml:lang="en">was Generated By</skos:prefLabel>
    <skos:definition xml:lang="en">provides the business context for, the creation of the dataset.</skos:definition>
  </rdf:Description>
  <rdf:Description rdf:about="http://purl.org/dc/terms/LicenseDocument">
    <rdf:type rdf:resource="http://www.w3.org/2002/07/owl#Class"/>
    <skos:prefLabel xml:lang="en">License Document</skos:prefLabel>
    <skos:definition xml:lang="en">A legal document giving official permission to do something with a resource.</skos:definition>
  </rdf:Description>
  <rdf:Description rdf:about="http://www.w3.org/2004/02/skos/core#prefLabel">
    <rdf:type rdf:resource="http://www.w3.org/2002/07/owl#DatatypeProperty"/>
    <skos:prefLabel xml:lang="en">pref Label</skos:prefLabel>
  </rdf:Description>
  <rdf:Description rdf:about="http://www.w3.org/ns/odrl/2/Policy">
    <rdf:type rdf:resource="http://www.w3.org/2002/07/owl#Class"/>
    <skos:prefLabel xml:lang="en">Policy</skos:prefLabel>
    <skos:definition xml:lang="en">A non-empty group of Permissions and/or Prohibitions.</skos:definition>
  </rdf:Description>
  <rdf:Description rdf:about="http://purl.org/dc/terms/license">
    <rdf:type rdf:resource="http://www.w3.org/2002/07/owl#ObjectProperty"/>
    <skos:prefLabel xml:lang="en">license</skos:prefLabel>
    <skos:definition xml:lang="en">A licence under which the Distribution is made available.</skos:definition>
  </rdf:Description>
  <rdf:Description rdf:about="http://www.w3.org/ns/adms#sample">
    <rdf:type rdf:resource="http://www.w3.org/2002/07/owl#ObjectProperty"/>
    <skos:prefLabel xml:lang="en">sample</skos:prefLabel>
    <skos:definition xml:lang="en">A sample distribution of the dataset. Usage: DCAT-AP-LU provides additional usage guidance for the use of this property in providing data dictionaries as part of dataset descriptions.</skos:definition>
  </rdf:Description>
  <rdf:Description rdf:about="http://www.w3.org/ns/adms#Identifier">
    <rdf:type rdf:resource="http://www.w3.org/2002/07/owl#Class"/>
    <skos:prefLabel xml:lang="en">Identifier</skos:prefLabel>
  </rdf:Description>
</rdf:RDF>
